chore: address warnings in core

src/Init/Data/List/Basic.lean
@@ -968,10 +968,11 @@ abbrev extract (l : List α) (start : Nat := 0) (stop : Nat := l.length) : List 
 @[simp] theorem extract_eq_take_drop {l : List α} {start stop : Nat} :
     l.extract start stop = (l.drop start).take (stop - start) := rfl
 
-set_option linter.defProp false in
-set_option linter.missingDocs false in
 @[deprecated extract_eq_take_drop (since := "2026-02-06")]
-def extract_eq_drop_take := @extract_eq_take_drop
+theorem extract_eq_drop_take {l : List α} {start stop : Nat} :
+    l.extract start stop = (l.drop start).take (stop - start) :=
+  extract_eq_take_drop
+
 
 /-! ### takeWhile -/
 
